Interpretation function for SMTLib.term

theories/SMTLib.v
@@ -41,6 +41,138 @@ Section SMTLib.
   | Term_And : term -> term -> term
   .
 
+
+  (* To be able to interpret function symbol application, we introduce
+     an informative cast between sorts
+
+     See
+     https://www.lri.fr/~keller/Documents-recherche/Publications/thesis13.pdf
+     Sec.3.2.2 *)
+  Section Cast.
+    Definition cast_result (A:Type) (n m:A) :=
+      option (forall (P:A -> Type), P n -> P m).
+    Definition idcast (A:Type) (n:A) : cast_result A n n :=
+      Some (fun P x => x).
+    Arguments idcast {A n}.
+
+    Fixpoint nat_cast (n m:nat) : cast_result nat n m :=
+      match n, m with
+      | O, O => idcast
+      | S n, S m =>
+          match nat_cast n m with
+          | Some k => Some (fun P => k (fun x => P (S x)))
+          | None => None
+          end
+      | _, _ => None
+      end.
+
+    Lemma nat_cast_refl:
+      forall n, nat_cast n n = idcast.
+    Proof. induction n as [ |n IHn]; simpl; try rewrite IHn; auto. Qed.
+
+    Fixpoint cast (A B:sort) : cast_result sort A B :=
+      match A, B return cast_result sort A B with
+      | Sort_Bool, Sort_Bool => idcast
+      | Sort_Int, Sort_Int => idcast
+      | Sort_Uninterpreted n1, Sort_Uninterpreted n2 =>
+          match nat_cast n1 n2 with
+          | Some k => Some (fun P => k (fun x => P (Sort_Uninterpreted x)))
+          | None => None
+          end
+      | _, _ => None
+      end.
+
+    Lemma cast_refl:
+      forall s, cast s s = idcast.
+    Proof. destruct s as [ | |n]; simpl; auto. now rewrite nat_cast_refl. Qed.
+
+  End Cast.
+
+
+  (* Interpretation *)
+  Section Interpretation.
+
+    (* Interpretation of sorts *)
+    Variable interp_sort_sym : sort_sym -> Type.
+
+    Definition interp_sort (s:sort) : Type :=
+      match s with
+      | Sort_Bool => bool
+      | Sort_Int => Z
+      | Sort_Uninterpreted sy => interp_sort_sym sy
+      end.
+
+    (* Interpretation of function types *)
+    Fixpoint interp_fun_type (dom:list sort) (codom:sort) : Type :=
+      match dom with
+      | nil => interp_sort codom
+      | s::dom => (interp_sort s) -> (interp_fun_type dom codom)
+      end.
+
+    (* Applying function symbols *)
+    Fixpoint apply_fun (dom:list sort) (codom:sort) :
+      (interp_fun_type dom codom) ->
+      (list (option {A:sort & interp_sort A})) ->
+      option (interp_sort codom) :=
+      match dom return
+            (interp_fun_type dom codom) ->
+            (list (option {A:sort & interp_sort A})) ->
+            option (interp_sort codom)
+      with
+      | nil => fun f _ => Some f
+      | s::dom => fun f arg =>
+                  match arg with
+                  | (Some (existT _ s' a))::arg =>
+                      match cast s' s with
+                      | Some k => apply_fun dom codom (f (k _ a)) arg
+                      | None => None
+                      end
+                  | _ => None
+                  end
+      end.
+
+    (* Interpretation of terms *)
+    Variable interp_fun_sym :
+      nat -> forall (dom:list sort) (codom:sort), interp_fun_type dom codom.
+
+    Fixpoint interp_term (t:term) : option {A : sort & interp_sort A} :=
+      match t with
+      | Term_Fun (n, (dom, codom)) arg =>
+          match apply_fun dom codom (interp_fun_sym n dom codom)
+                  (List.map interp_term arg)
+          with
+          | Some i => Some (existT _ codom i)
+          | None => None
+          end
+      | Term_Int z => Some (existT _ Sort_Int z)
+      | Term_Geq t1 t2 =>
+          match interp_term t1, interp_term t2 with
+          | Some (existT _ Sort_Int z1), Some (existT _ Sort_Int z2) =>
+              Some (existT _ Sort_Bool (z1 >=? z2)%Z)
+          | _, _ => None
+          end
+      | Term_Eq t1 t2 =>
+          match interp_term t1, interp_term t2 with
+          | Some (existT _ Sort_Int z1), Some (existT _ Sort_Int z2) =>
+              Some (existT _ Sort_Bool (z1 =? z2)%Z)
+          | _, _ => None
+          end
+      | Term_And t1 t2 =>
+          match interp_term t1, interp_term t2 with
+          | Some (existT _ Sort_Bool b1), Some (existT _ Sort_Bool b2) =>
+              Some (existT _ Sort_Bool (b1 && b2)%bool)
+          | _, _ => None
+          end
+      end.
+
+    Definition interp_formula (t:term) : bool :=
+      match interp_term t with
+      | Some (existT _ Sort_Bool b) => b
+      | _ => true
+      end.
+
+  End Interpretation.
+
 End SMTLib.
 
 
